Add runlength for list of bytes

RunLength.v
@@ -4,8 +4,12 @@ Require Import Coq.Init.Nat.
 Require Import Omega.
 Require Import Coq.Bool.Bool.
 Require Import Recdef.
+Require Import Instances.
+Require Import NatEncode.
+Require Import compcert.lib.Integers.
+Require Import Coqlib.
 
-Require Import VST.fcf.EqDec.
+Require Import fcf.EqDec.
 
 Section RunLength.
 
@@ -13,154 +17,242 @@ Section RunLength.
   Open Scope nat_scope.
   Open Scope eq_scope.
 
-  Generalizable Variable A.
-  Context `{ED : EqDec A}.
+  Context `{A: Set}.
 
-  (* maxRun is the maximum length of a run. Useful if we want to
-       later encode the run-length encoded list in some fixed-size
-       binary representation, so we have a limit on the largest
-       representable number. *)
-  Variable maxRun : nat.
-  Hypothesis HMaxRunPos : maxRun > 0.
+  Section Encode.
+    Context `{ED : EqDec A}.
 
-  (* Add one element to a run-length encoded list l. *)
-  Definition run_length_cons (x: A) (l: list (A * nat)) :=
-    match l with
-    | nil => [(x,1)]
-    | (y,count)::tl =>
-      if (x ?= y) && (count <? maxRun)
-      then (x, Nat.succ count) :: tl
-      else (x,1) :: (y, count) :: tl
-    end.
+    (* modulus is the an upper bound on the length of a run. Useful if
+       we want to later encode the run-length encoded list in some
+       fixed-size binary representation, so we have a limit on the
+       largest representable number. *)
+    Variable modulus : nat.
+    Hypothesis HModulusPos : modulus > 1.
 
-  (* Run length encode an entire list. *)
-  Definition run_length_encode :=
-    List.fold_right run_length_cons [].
+    (* Add one element to a run-length encoded list l. *)
+    Definition run_length_cons (x: A) (l: list (A * nat)) :=
+      match l with
+      | nil => [(x,1)]
+      | (y,count)::tl =>
+        if (x ?= y) && (Nat.succ count <? modulus)
+        then (x, Nat.succ count) :: tl
+        else (x,1) :: (y, count) :: tl
+      end.
 
-  (* A useful lemma to break down proofs about run_length_cons into 4 cases:
+    (* Run length encode an entire list. *)
+    Definition run_length_encode : list A -> list (A * nat) :=
+      List.fold_right run_length_cons [].
+
+    (* A useful lemma to break down proofs about run_length_cons into 4 cases:
      - l = []
-     - x = hd and count < maxRun
-     - x = hd and count >= maxRun
+     - x = hd and count+1 < modulus
+     - x = hd and count+1 >= modulus
      - x <> hd
-   *)
-  Lemma run_length_cons_cases :
-    (* P is a relation between the inputs of run_length_cons and its output *)
-    forall x l (P: A -> list (A * nat) -> list (A * nat) -> Prop),
-      (* l = 0 *)
-      P x [] [(x, 1)] ->
-      (* x = hd and count < maxRun *)
-      (forall hd count tl,
-          x = hd -> count < maxRun ->
-          P x ((hd,count)::tl) ((hd, Nat.succ count)::tl)) ->
-      (* x = hd and count >= maxRun *)
-      (forall hd count tl,
-          x = hd -> count >= maxRun ->
-          P x ((hd,count)::tl) ((x,1)::(hd,count)::tl)) ->
-      (* x <> hd *)
-      (forall hd count tl,
-          x <> hd ->
-          P x ((hd,count)::tl) ((x,1)::(hd,count)::tl)) ->
-      P x l (run_length_cons x l).
-  Proof.
-    intros x l P HBase HEq HOver HNew.
-    induction l as [| p tl].
-    - apply HBase.
-    - destruct p as [hd count].
-      destruct (EqDec_dec _ x hd) as [Eq | Neq].
-      + simpl. rewrite (proj2 (eqb_leibniz _ _) Eq).
-        destruct (le_lt_dec maxRun count) as [ Ge | Lt ].
-        * assert (Ge': count >= maxRun) by omega.
-          rewrite (proj2 (Nat.ltb_ge _ _) Ge'). simpl.
-          apply HOver; auto.
-        * rewrite (proj2 (Nat.ltb_lt _ _) Lt). simpl.
-          subst x. apply HEq; auto.
-      + simpl. rewrite (proj2 (eqb_false_iff _ _ _) Neq).
-        rewrite andb_false_l.
-        apply HNew; auto.
-  Qed.
+     *)
+    Lemma run_length_cons_cases :
+      (* P is a relation between the inputs of run_length_cons and its output *)
+      forall x l (P: A -> list (A * nat) -> list (A * nat) -> Prop),
+        (* l = 0 *)
+        P x [] [(x, 1)] ->
+        (* x = hd and count < modulus *)
+        (forall hd count tl,
+            x = hd -> Nat.succ count < modulus ->
+            P x ((hd,count)::tl) ((hd, Nat.succ count)::tl)) ->
+        (* x = hd and count >= modulus *)
+        (forall hd count tl,
+            x = hd -> Nat.succ count >= modulus ->
+            P x ((hd,count)::tl) ((x,1)::(hd,count)::tl)) ->
+        (* x <> hd *)
+        (forall hd count tl,
+            x <> hd ->
+            P x ((hd,count)::tl) ((x,1)::(hd,count)::tl)) ->
+        P x l (run_length_cons x l).
+    Proof.
+      intros x l P HBase HEq HOver HNew.
+      induction l as [| p tl].
+      - apply HBase.
+      - destruct p as [hd count].
+        destruct (EqDec_dec _ x hd) as [Eq | Neq].
+        + simpl. rewrite (proj2 (eqb_leibniz _ _) Eq).
+          destruct (le_lt_dec modulus (Nat.succ count)) as [ Ge | Lt ].
+          * assert (Ge': Nat.succ count >= modulus) by omega.
+            rewrite (proj2 (Nat.ltb_ge _ _) Ge'). simpl.
+            apply HOver; auto.
+          * rewrite (proj2 (Nat.ltb_lt _ _) Lt). simpl.
+            subst x. apply HEq; auto.
+        + simpl. rewrite (proj2 (eqb_false_iff _ _ _) Neq).
+          rewrite andb_false_l.
+          apply HNew; auto.
+    Qed.
 
-  (* run_bounded asserts that every run in l is less than or equal to
-     maxRun *)
-  Definition run_bounded (l: list (A * nat)) :=
-    Forall (fun x => x <= maxRun) (map snd l).
+    (* run_bounded asserts that every run in l is less than or equal to
+     modulus *)
+    Definition run_bounded (l: list (A * nat)) :=
+      Forall (fun x => x < modulus) (map snd l).
 
-  (* run_length_cons preserves run_bounded *)
-  Lemma run_length_cons_bounded : forall x l,
-      run_bounded l -> run_bounded (run_length_cons x l).
-  Proof.
-    intros x l.
-    apply run_length_cons_cases;
-      try (intros hd count tl HEq HLT HInd);
-      simpl; try (inversion HInd; subst); econstructor; auto; simpl; try omega.
-  Qed.
+    (* run_length_cons preserves run_bounded *)
+    Lemma run_length_cons_bounded : forall x l,
+        run_bounded l -> run_bounded (run_length_cons x l).
+    Proof.
+      intros x l.
+      apply run_length_cons_cases;
+        try (intros hd count tl HEq HLT HInd);
+        simpl; try (inversion HInd; subst); econstructor; auto; simpl; try omega.
+    Qed.
 
-  (* run_length_encode preserves run_bounded *)
-  Theorem run_length_bounded : forall l,
-      run_bounded (run_length_encode l).
-  Proof.
-    induction l.
-    - econstructor.
-    - unfold run_length_encode. simpl.
-      apply run_length_cons_bounded; auto.
-  Qed.
+    (* run_length_encode preserves run_bounded *)
+    Theorem run_length_bounded : forall l,
+        run_bounded (run_length_encode l).
+    Proof.
+      induction l.
+      - econstructor.
+      - unfold run_length_encode. simpl.
+        apply run_length_cons_bounded; auto.
+    Qed.
+  End Encode.
 
-  (* We define a measure that will decrease on each recursive call to
+  Section Decode.
+    (* We define a measure that will decrease on each recursive call to
      run_length_decode, so that we can prove that it terminates. To
      that end, we measure the cons cell itself as 1 so that the
      measure decreases when we remove a cons cell with a 0 run.*)
-  Fixpoint run_length_measure (l : list (A * nat)) :=
-    match l with
-    | [] => 0
-    | (_,count)::tl =>
-      if count ?= 0
-      then 1 + run_length_measure tl
-      else 1 + count + run_length_measure tl
-    end.
+    Fixpoint run_length_measure (l : list (A * nat)) :=
+      match l with
+      | [] => 0
+      | (_,count)::tl =>
+        if count ?= 0
+        then 1 + run_length_measure tl
+        else 1 + count + run_length_measure tl
+      end.
 
-  (* decode a run-length encoded list *)
-  Function run_length_decode (l : list (A * nat)) { measure run_length_measure l } :=
-    match l with
-    | [] => []
-    | (x,count)::tl =>
-      if 0 <? count
-      then x :: run_length_decode ((x, Nat.pred count) :: tl)
-      else run_length_decode tl
-    end.
-  Proof.
-    - intros l p tl x count HP HL HLT. simpl.
-      destruct (Nat.eq_dec 1 count) as [Eq | NEq].
-      + subst. simpl. omega.
-      + apply Nat.ltb_lt in HLT.
-        assert (HLT': 0 < Nat.pred count) by omega.
-        rewrite (proj2 (Nat.leb_gt _ _) HLT').
-        rewrite (proj2 (Nat.leb_gt _ _) HLT). simpl.
-        omega.
-    - intros l p tl x count HP HL HLT. simpl.
-      rewrite Nat.ltb_antisym in HLT.
-      rewrite (proj1 (negb_false_iff _) HLT).
-      simpl. omega.
-  Defined.
+    (* decode a run-length encoded list *)
+    Function run_length_decode (l : list (A * nat)) { measure run_length_measure l } :=
+      match l with
+      | [] => []
+      | (x,count)::tl =>
+        if 0 <? count
+        then x :: run_length_decode ((x, Nat.pred count) :: tl)
+        else run_length_decode tl
+      end.
+    Proof.
+      - intros l p tl x count HP HL HLT. simpl.
+        destruct (Nat.eq_dec 1 count) as [Eq | NEq].
+        + subst. simpl. omega.
+        + apply Nat.ltb_lt in HLT.
+          assert (HLT': 0 < Nat.pred count) by omega.
+          rewrite (proj2 (Nat.leb_gt _ _) HLT').
+          rewrite (proj2 (Nat.leb_gt _ _) HLT). simpl.
+          omega.
+      - intros l p tl x count HP HL HLT. simpl.
+        rewrite Nat.ltb_antisym in HLT.
+        rewrite (proj1 (negb_false_iff _) HLT).
+        simpl. omega.
+    Defined.
+  End Decode.
 
   (* run_length_decode-ing the result of a run_length_cons is the same
      as regular cons followed by run_length_decode *)
-  Lemma run_length_cons_invert : forall x l,
-      run_length_decode (run_length_cons x l) = x :: run_length_decode l.
+  Lemma run_length_cons_invert `{EqDec A}: forall modulus x l,
+      modulus > 1 ->
+      run_length_decode (run_length_cons modulus x l) = x :: run_length_decode l.
   Proof.
-    intros x l.
+    intros modulus x l HMaxRunPos.
     apply run_length_cons_cases;
       intros; simpl;
         do 2 (try (rewrite run_length_decode_equation);
-              simpl; subst; try reflexivity).
+              simpl; subst; auto; try reflexivity).
   Qed.
 
   (* run_length_decode undoes run_length_encode *)
-  Theorem run_length_invert : forall l,
-      run_length_decode (run_length_encode l) = l.
+  Theorem run_length_invert `{EqDec A}: forall modulus l,
+      modulus > 1 ->
+      run_length_decode (run_length_encode modulus l) = l.
   Proof.
+    intros modulus l HMaxRunPos; revert l.
     induction l as [| hd tl].
     - rewrite run_length_decode_equation. reflexivity.
-    - simpl. rewrite run_length_cons_invert.
+    - simpl. rewrite run_length_cons_invert; auto.
       f_equal. apply IHtl.
   Qed.
 
 End RunLength.
+
+Section Run_Encoding.
+
+  Open Scope nat_scope.
+
+  Generalizable Variable A.
+  Context `{NE : NatEncode A}.
+
+  Definition encode_runs : list (A * nat) -> list A :=
+    let flatten_run p : list A :=
+        match p with (x, count) => [x; encode count] end
+    in flat_map flatten_run.
+
+  Fixpoint decode_runs (l: list A) : list (A * nat) :=
+    match l with
+    | x::count::tl => (x, decode count) :: decode_runs tl
+    | _ => []
+    end.
+
+  Theorem encode_runs_inverse : forall l,
+      Forall (fun x => x < modulus) (map snd l) ->
+      decode_runs (encode_runs l) = l.
+  Proof.
+    induction l.
+    - intros; reflexivity.
+    - intros HBounded.
+      inversion HBounded; subst; clear HBounded.
+      destruct a as [x count]. simpl.
+      rewrite IHl; auto. do 2 f_equal.
+      apply nat_encode_inverse.
+      simpl in H1; auto.
+  Qed.
+
+End Run_Encoding.
+
+Section Bytes.
+
+  Local Definition modulus := Z.to_nat Byte.modulus.
+  Lemma two_p_gt_ONE : forall x,
+      0 < x -> two_p x > 1.
+  Proof.
+    intros.
+    replace 1 with (two_p 0) by reflexivity.
+    apply Z.lt_gt.
+    apply two_p_monotone_strict.
+    omega.
+  Qed.
+
+  Lemma modulus_gt_one : 1 < Byte.modulus.
+    rewrite Byte.modulus_power.
+    apply Z.gt_lt. apply two_p_gt_ONE.
+    generalize Byte.wordsize_pos; omega.
+  Qed.
+
+  Open Scope nat_scope.
+
+  Theorem HMaxRunPos : modulus > 1.
+  Proof.
+    unfold modulus.
+    pose proof modulus_gt_one.
+    apply (Z2Nat.inj_lt 1 _); try omega.
+  Qed.
+
+  Definition run_length_encode_bytes (l: list byte) : list byte :=
+    encode_runs (run_length_encode modulus l).
+
+  Definition run_length_decode_bytes (l: list byte) : list byte :=
+    run_length_decode (decode_runs l).
+
+  Theorem run_length_bytes_invert : forall l,
+      run_length_decode_bytes (run_length_encode_bytes l) = l.
+  Proof.
+    intros.
+    pose proof HMaxRunPos.
+    unfold run_length_encode_bytes, run_length_decode_bytes.
+    rewrite encode_runs_inverse.
+    rewrite run_length_invert; auto.
+    apply run_length_bounded; auto.
+  Qed.
+End Bytes.
