NatEncode.v
@@ -1,0 +1,38 @@
+Require compcert.lib.Integers.
+Require Import Coqlib.
+
+Open Scope nat_scope.
+Class NatEncode (A : Set) := {
+  modulus : nat;
+  encode : nat -> A;
+  decode : A -> nat;
+  nat_encode_inverse : forall x, x < modulus -> decode (encode x) = x
+}.
+Close Scope nat_scope.
+
+Theorem int_nat_encode : forall {I: Set} {modulus: Z} {repr: Z -> I} {unsigned: I -> Z},
+    modulus > 0 ->
+    (forall x, unsigned (repr x) = x mod modulus) ->
+    NatEncode I.
+Proof.
+  intros I modulus repr unsigned modulus_pos unsigned_repr_eq.
+  eapply (Build_NatEncode I
+            (Z.to_nat modulus)
+            (fun x => repr (Z.of_nat x))
+            (fun x => Z.to_nat (unsigned x))).
+  intros.
+  rewrite unsigned_repr_eq.
+  rewrite <- Nat2Z.id in H at 1.
+  rewrite <- Z2Nat.inj_lt in H; try omega.
+  rewrite Z.mod_small; try omega.
+  apply Nat2Z.id.
+Defined.
+
+Instance Byte_NatEncode : NatEncode Integers.Byte.int
+  := int_nat_encode Integers.Byte.modulus_pos Integers.Byte.unsigned_repr_eq.
+Instance Int_NatEncode : NatEncode Integers.Int.int
+  := int_nat_encode Integers.Int.modulus_pos Integers.Int.unsigned_repr_eq.
+Instance Int64_NatEncode : NatEncode Integers.Int64.int
+  := int_nat_encode Integers.Int64.modulus_pos Integers.Int64.unsigned_repr_eq.
+Instance Ptrofs_NatEncode : NatEncode Integers.Ptrofs.int
+  := int_nat_encode Integers.Ptrofs.modulus_pos Integers.Ptrofs.unsigned_repr_eq.
