Makefile
@@ -1,11 +1,18 @@
-COQC := coqc `cat _CoqProject`
+COQFLAGS := `cat _CoqProject`
+COQC := coqc $(COQFLAGS)
 
 all: RunLength.vo
 
 clean:
 	fd --no-ignore-vcs -e vo -e glob -x rm {}
 
-RunLength.vo: VST/fcf/EqDec.vo
+RunLength.vo: Instances.vo NatEncode.vo VST/fcf/EqDec.vo
+Instances.vo: VST/fcf/EqDec.vo VST/compcert/lib/Integers.vo
+NatEncode.vo: VST/compcert/lib/Integers.vo
+
+
+VST/%.vo: VST/%.v
+	$(MAKE) -C VST COQFLAGS="$(COQFLAGS)" $(patsubst VST/%,%,$@)
 
 %.vo: %.v
 	$(COQC) $<
